hw1 done

pset01_ProgramAnalysis/Pset1.v
@@ -16,8 +16,11 @@ Require Import Frap Pset1Sig.
 (* Define [Neg] so that it implements Boolean negation, which flips
  * the truth value of a Boolean value.
  *)
-Definition Neg (b : bool) : bool.
-Admitted.
+Definition Neg (b : bool) : bool := 
+  match b with
+    | true => false
+    | false => true
+  end.
 
 (* For instance, the negation of [true] should be [false].
  * This proof should follow from reducing both sides of the equation
@@ -25,8 +28,9 @@ Admitted.
  *)
 Theorem Neg_true : Neg true = false.
 Proof.
-Admitted.
-
+simplify.
+equality.
+Qed.
 (* Negation should be involutive, meaning that if we negate
  * any Boolean value twice, we should get the original value back.
 
@@ -36,39 +40,51 @@ Admitted.
  *)
 Theorem Neg_involutive : forall b : bool, Neg (Neg b) = b.
 Proof.
-Admitted.
+  simplify.
+  cases b; try (simplify; equality).
+Qed.
 
 (* Define [And] so that it implements Boolean conjunction. That is,
  * the result value should be [true] exactly when both inputs
  * are [true].
  *)
-Definition And (x y : bool) : bool.
-Admitted.
+Definition And (x y : bool) : bool := 
+  match x,y with
+    | true, true => true
+    | _, _ => false
+  end.
 
 (* Here are a couple of examples of how [And] should act on
  * concrete inputs.
  *)
 Theorem And_true_true : And true true = true.
 Proof.
-Admitted.
+simplify.
+equality.
+Qed.
 
 Theorem And_false_true : And false true = false.
 Proof.
-Admitted.
+simplify.
+equality.
+Qed.
 
 (* Prove that [And] is commutative, meaning that switching the order
  * of its arguments doesn't affect the result.
  *)
 Theorem And_comm : forall x y : bool, And x y = And y x.
 Proof.
-Admitted.
-
+simplify.
+cases x; (cases y; simplify; equality).
+Qed.
 (* Prove that the conjunction of a Boolean value with [true]
  * doesn't change that value.
  *)
 Theorem And_true_r : forall x : bool, And x true = x.
 Proof.
-Admitted.
+simplify.
+cases x; simplify; equality.
+Qed.
 
 (* In the second part of this assignment, we will work with a simple language
  * of imperative arithmetic programs that sequentially apply operations
@@ -79,48 +95,92 @@ Admitted.
 
 Print Prog.
 
+
 (* Define [run] such that [run p n] gives the final state
  * that running the program [p] should result in, when the
  * initial state is [n].
  *)
-Fixpoint run (p : Prog) (initState : nat) : nat.
-Admitted.
+Fixpoint run (p : Prog) (initState : nat) : nat :=
+  match p with
+    | Done => initState
+    | AddThen e1 p1 => run p1 (initState + e1)
+    | MulThen e2 p2 => run p2 (initState * e2)
+    | DivThen e3 p3 => run p3 (initState / e3)
+    | VidThen e4 p4 => run p4 (e4 / initState)
+    | SetToThen e5 p5 => run p5 e5
+end.
 
+Print Prog.
+Example test := (MulThen 5 (AddThen 2 Done)).
+Compute run test 2.
 Theorem run_Example1 : run Done 0 = 0.
 Proof.
-Admitted.
+simplify.
+equality.
+Qed.
 
 Theorem run_Example2 : run (MulThen 5 (AddThen 2 Done)) 1 = 7.
 Proof.
-Admitted.
+  simplify.
+  equality.
+Qed.
+
 
 Theorem run_Example3 : run (SetToThen 3 (MulThen 2 Done)) 10 = 6.
 Proof.
-Admitted.
-
+simplify.
+equality.
+Qed.
 (* Define [numInstructions] to compute the number of instructions
  * in a program, not counting [Done] as an instruction.
  *)
-Fixpoint numInstructions (p : Prog) : nat.
-Admitted.
+Fixpoint numInstructions (p : Prog) : nat :=
+  match p with 
+    | Done => 0
+    | AddThen e1 p1   => 1 + numInstructions (p1)
+    | MulThen e1 p1   => 1 + numInstructions (p1)
+    | DivThen e1 p1   => 1 + numInstructions (p1)
+    | VidThen e1 p1   => 1 + numInstructions (p1)
+    | SetToThen e1 p1 => 1 + numInstructions (p1)
+  end.
 
 Theorem numInstructions_Example :
   numInstructions (MulThen 5 (AddThen 2 Done)) = 2.
 Proof.
-Admitted.
+  simplify.
+  equality.
+Qed.
 
 (* Define [concatProg] such that [concatProg p1 p2] is the program
  * that first runs [p1] and then runs [p2].
  *)
-Fixpoint concatProg (p1 p2 : Prog) : Prog.
-Admitted.
+Fixpoint concatProg (p1 p2 : Prog) : Prog := 
+  match p1 with
+    | Done => p2
+    | AddThen e1 res => AddThen e1 (concatProg res p2)
+    | MulThen e1 res => MulThen e1 ( concatProg res p2)
+    | DivThen e1 res => DivThen e1 ( concatProg res p2)
+    | VidThen e1 res => VidThen e1 ( concatProg res p2)
+    | SetToThen e1 res => SetToThen e1 (concatProg res p2)
+  end.
+
+Example a := concatProg (AddThen 1 Done) (MulThen 2 Done). 
+Compute a.
 
 Theorem concatProg_Example :
      concatProg (AddThen 1 Done) (MulThen 2 Done)
      = AddThen 1 (MulThen 2 Done).
 Proof.
-Admitted.
+simplify.
+equality.
+Qed.
 
+Theorem concat_base
+  : forall (p1: Prog), concatProg p1 Done = p1.
+Proof.
+  simplify.
+  induct p1; simplify; equality.
+Qed.
 (* Prove that the number of instructions in the concatenation of
  * two programs is the sum of the number of instructions in each
  * program.
@@ -129,8 +189,9 @@ Theorem concatProg_numInstructions
   : forall (p1 p2 : Prog), numInstructions (concatProg p1 p2)
                       = numInstructions p1 + numInstructions p2.
 Proof.
-Admitted.
-
+simplify.
+induction p1; simplify; equality; simplify; rewrite IHp1; equality.
+Qed.
 (* Prove that running the concatenation of [p1] with [p2] is
    equivalent to running [p1] and then running [p2] on the
    result. *)
@@ -139,8 +200,8 @@ Theorem concatProg_run
     run (concatProg p1 p2) initState =
     run p2 (run p1 initState).
 Proof.
-Admitted.
-
+induct p1; simplify; equality.
+Qed.
 (* Read this definition and understand how division by zero is handled. *)
 Fixpoint runPortable (p : Prog) (state : nat) : bool * nat :=
   match p with
@@ -158,14 +219,148 @@ Fixpoint runPortable (p : Prog) (state : nat) : bool * nat :=
   end.
 Arguments Nat.div : simpl never. (* you don't need to understand this line *)
 
+
+
+
+
+Lemma run_portable_helper: forall (p: Prog) (n: nat),
+  runPortable (DivThen 0 p) n = (false, n).
+Proof.
+  simplify.
+  cases (n);simplify; equality.
+Qed.
+
+Lemma run_portable_helper_vid: forall (p: Prog) (n: nat),
+  runPortable (VidThen n p) 0 = (false, 0).
+Proof.
+  simplify.
+  cases (n);simplify; equality.
+Qed.
+
+
+Lemma run_portable_helper2: forall (p: Prog) (n n2: nat),
+  n <> 0 -> runPortable (DivThen n p) n2 = runPortable p (n2 / n).
+Proof.
+  simplify.
+  cases (n ==n 0).
+  contradiction.
+  equality.
+Qed.
+
+
+Lemma run_portable_helper_vid2: forall (p: Prog) (n n2: nat),
+  n2 <> 0 -> runPortable (VidThen n p) n2 = runPortable p (n / n2).
+Proof.
+  simplify.
+  cases (n2 ==n 0).
+  contradiction.
+  equality.
+Qed.
+
+
+Lemma run_portable_helper3: forall(p: Prog) (n s0 s1: nat),  
+   (runPortable (DivThen n p) s0 = (true, s1)) -> n <> 0.
+Proof.
+intros.
+cases n.
+assert(H2: runPortable (DivThen 0 p) s0 = (false, s0)).
+apply run_portable_helper.
+rewrite H in H2.
+equality.
+linear_arithmetic.
+Qed.
+
+Lemma run_portable_helper_vid3: forall(p: Prog) (n s0 s1: nat),  
+   (runPortable (VidThen n p) s0 = (true, s1)) -> s0 <> 0.
+Proof.
+intros.
+cases s0.
+assert(H2: runPortable (VidThen n p) 0 = (false, 0)).
+apply run_portable_helper_vid.
+rewrite H in H2.
+equality.
+linear_arithmetic.
+Qed.
+
+
 (* Prove that running the concatenation [p] using [runPortable]
    coincides with using [run], as long as [runPortable] returns
    [true] to confirm that no divison by zero occurred. *)
+   
 Lemma runPortable_run : forall p s0 s1,
   runPortable p s0 = (true, s1) -> run p s0 = s1.
 Proof.
-Admitted.
+intros.
+induct p; try(simplify; equality); try(apply IHp in H; simplify; try(rewrite plus_comm); try(rewrite mult_comm); try apply H).
 
+apply IHp.
+rewrite <- H.
+rewrite run_portable_helper2.
+equality.
+assert(H2: runPortable (DivThen n p) s0 = (true, s1) -> n <> 0).
+apply run_portable_helper3.
+apply H2.
+apply H.
+
+apply IHp.
+rewrite <- H.
+rewrite run_portable_helper_vid2.
+equality.
+assert(H2: runPortable (VidThen n p) s0 = (true, s1) -> s0 <> 0).
+apply run_portable_helper_vid3.
+apply H2.
+apply H.
+
+Qed.
+
+Fixpoint validate_helper p (b : bool) :=
+    match p with
+    | Done => true
+    | AddThen n p => if n ==n 0 then validate_helper p b else validate_helper p true
+    | MulThen n p => if n ==n 0 then validate_helper p false else validate_helper p b
+    | DivThen n p => if n ==n 0 then false else (if b then validate_helper p (Nat.eqb n 1) else validate_helper p false)
+    | VidThen n p => if b then validate_helper p false else false
+    | SetToThen n p => if n ==n 0 then validate_helper p false else validate_helper p true
+    end. 
+
+
+Definition validate (p : Prog) : bool :=
+  validate_helper p false.
+
+
+(*Lemma validate_sound_helper: forall (p: Prog), validate p = true -> forall s, fst(runPortable p s) = true -> fst(runPortable p 0) = true.
+induct p; simplify; try(apply IHp); try(equality).
+unfold validate in IHp.
+apply IHp.
+Qed.*)
+
+
+(*Lemma b : forall (p: Prog)(n: nat), fst (runPortable p (n)) = true <-> (runPortable p n = (true, run p n)).
+Proof.
+  induct p; simplify; try (apply IHp in H); try(rewrite <- plus_comm); try(rewrite <- mult_comm);
+  try(equality); try(rewrite plus_comm in H); try(rewrite mult_comm in H); try(assumption);
+  try(cases(n ==n 0); cases (n0 ==n 0));simplify; try(equality); try(rewrite IHp); try(equality).
+Qed.
+
+Lemma concat_portable : forall p1 p2 n, runPortable (concatProg p1 p2) n
+        = (let (x, answer) := runPortable p1 n in if x then runPortable p2 answer else (x,answer)).
+Proof.
+  induct p1; try equality; simplify; try apply IHp1; try equality; try( cases (n ==n 0); cases (n0 ==n 0);
+  try equality;
+  simplify;
+  apply IHp1).
+Qed.
+*)
+  (* If a clear plan hasn't emerged in 10 minutes (or if you get stuck later),
+ * take a look at the hints for this pset on the course web site.
+ * It is not expected that this pset is doable for everyone without the hints,
+ * but some planning is required for successful proof.
+ * In particular, repeatedly trying out different combinations of tactics
+ * and ideas from hints until something sticks can go on for arbitrarily long
+ * with little insight and no success; just guessing a solution is unlikely.
+ * Thus, we encourage you to take your time thinking, look at the hints when
+ * necessary, and only jump into coding when you have some idea why it should
+ * succeed. Some may call Coq a video game, but it is not a grinding contest. *)
 
 (* The final goal of this pset is to implement [validate : Prog -> bool]
    such that if this function returns [true], the program would not trigger
@@ -185,6 +380,7 @@ Example runPortable_bad : let n := 0 in
   runPortable badProgram1 n = (false, 0).
 Proof. simplify. equality. Qed.
 
+
 Definition badProgram2 := AddThen 1 (DivThen 0 Done).
 Example runPortable_bad2 : forall n,
   runPortable badProgram2 n = (false, 1+n).
@@ -202,33 +398,151 @@ Definition goodProgram7 := AddThen 1 (DivThen 1 (DivThen 1 (VidThen 1 Done))).
  * feel free to just code away. Our solution uses one intermediate definition
  * and one intermediate lemma in the soundness proof -- both of which are more
  * sophisticated than the top-level versions given here. *)
+Example validate1 : validate goodProgram1 = true. Proof. equality. Qed.
+Example validate2 : validate goodProgram2 = true. Proof. equality. Qed.
+Example validate3 : validate goodProgram3 = true. Proof. equality. Qed.  
+Example validate4 : validate goodProgram4 = true. Proof. equality. Qed.
+Example validate5 : validate goodProgram5 = true. Proof. equality. Qed.
+Example validate6 : validate goodProgram6 = true. Proof. equality. Qed.
+Example validate7 : validate goodProgram7 = true. Proof. equality. Qed.
+Example validate8 : validate badProgram1 = false. Proof. equality. Qed.
+Example validate9 : validate badProgram2 = false. Proof. equality. Qed.
 
-Definition validate (p : Prog) : bool.
-Admitted.
 
-Example validate1 : validate goodProgram1 = true. Admitted.
-Example validate2 : validate goodProgram2 = true. Admitted.
-Example validate3 : validate goodProgram3 = true. Admitted.
-Example validate4 : validate goodProgram4 = true. Admitted.
-Example validate5 : validate goodProgram5 = true. Admitted.
-Example validate6 : validate goodProgram6 = true. Admitted.
-Example validate7 : validate goodProgram7 = true. Admitted.
+Lemma validate_sound_helper: forall p b, validate_helper p b = true ->
+     forall s : nat, (b = true -> s <> 0) ->
+     runPortable p s = (true, run p s).
+induct p; try(simplify); try(equality).
+rewrite plus_comm.
+simplify.
+cases (n ==n 0).
+apply IHp with (b:=b).
+assumption.
+rewrite e.
+simplify.
+apply H0 in H1.
+linear_arithmetic.
+apply IHp with (b:=true).
+assumption.
+simplify.
+linear_arithmetic.
 
-(* If a clear plan hasn't emerged in 10 minutes (or if you get stuck later),
- * take a look at the hints for this pset on the course web site.
- * It is not expected that this pset is doable for everyone without the hints,
- * but some planning is required for successful proof.
- * In particular, repeatedly trying out different combinations of tactics
- * and ideas from hints until something sticks can go on for arbitrarily long
- * with little insight and no success; just guessing a solution is unlikely.
- * Thus, we encourage you to take your time thinking, look at the hints when
- * necessary, and only jump into coding when you have some idea why it should
- * succeed. Some may call Coq a video game, but it is not a grinding contest. *)
 
+
+rewrite mult_comm.
+simplify.
+cases (n ==n 0).
+apply IHp with (b:=false).
+assumption.
+propositional.
+equality.
+apply IHp with (b:=b).
+assumption.
+
+simplify.
+apply H0 in H1.
+simplify.
+apply Nat.neq_mul_0.
+propositional.
+
+cases (n ==n 0).
+equality.
+cases b.
+apply IHp with (b:= Nat.eqb n 1).
+assumption.
+cases(Nat.eqb n 1). 
+intros.
+apply Nat.eqb_eq in Heq.
+rewrite Heq.
+apply H0 in H1.
+rewrite Nat.div_1_r.
+assumption.
+propositional.
+equality.
+apply IHp with (b := false) (s := s/n).
+assumption.
+propositional.
+equality.
+
+cases (s ==n 0).
+cases b.
+propositional.
+equality.
+cases b.
+apply IHp with (b := false) (s := n/s).
+assumption.
+propositional.
+equality.
+equality.
+
+cases (n ==n 0).
+apply IHp with (b := false) (s := n).
+assumption.
+propositional.
+equality.
+
+apply IHp with (b := true) (s := n).
+assumption.
+propositional.
+Qed.
+
+Hint Rewrite Nat.add_0_r.
 Lemma validate_sound : forall p, validate p = true ->
   forall s, runPortable p s = (true, run p s).
-Admitted.
+Proof.
+induct p; try(simplify); try(equality); try(rewrite plus_comm).
+unfold validate in IHp.
 
+apply validate_sound_helper with (s:=s) in H.
+simplify.
+assert(ejre: n + s = s + n).
+linear_arithmetic.
+rewrite <- ejre.
+rewrite <- ejre in H.
+trivial.
+propositional.
+equality.
+
+
+apply validate_sound_helper with (s:=s) in H.
+simplify.
+assumption.
+propositional.
+equality.
+
+cases (n ==n 0).
+apply validate_sound_helper with (s:=s) in H.
+simplify.
+rewrite e in H.
+simplify.
+rewrite e.
+apply H.
+propositional.
+equality.
+
+apply validate_sound_helper with (s:=s) in H.
+simplify.
+cases (n ==n 0).
+equality.
+apply H.
+
+propositional.
+equality.
+
+apply validate_sound_helper with (s:= s) in H.
+simplify.
+apply H.
+
+propositional.
+equality.
+
+apply validate_sound_helper with (s:= s) in H.
+simplify.
+apply H.
+
+propositional.
+equality.
+Qed.
 (* Here is the complete list of commands used in one possible solution:
   - Search, for example Search (_ + 0).
   - induct, for example induct x
